% Begin section ----------------------------------------------------------------
\section{Question 4}

% Only part --------------------------------------------------------------------
\begin{frame}{Question 4}

    This question is a lot of algebra and we won't go over all of it during this session. But keep in mind these formulas

    \begin{align*}
        \hat{\alpha} &= \bar{y} - \bar{x} \hat{\beta}
        \\
        \hat{\beta} &= \frac{\sum_{i=1}^n (x_i - \bar{x}) (y_i - \bar{y}) }{\sum_{i=1}^n (x_i - \bar{x})^2}
    \end{align*}

    Note that
    \begin{align*}
        \widehat{\operatorname{Var}} \begin{pmatrix} \hat{\alpha} \\ \hat{\beta} \end{pmatrix} &= s^2 \begin{bmatrix} n & n \bar{x} \\ n \bar{x} \sum_{i=1}^n x_i^2 \end{bmatrix}^{-1}
        \\
        &= \frac{SSR}{(n-2) \sum_{i=1}^n (x_i - \bar{x})^2} \begin{bmatrix} \frac{1}{n} \sum_{i=1}^n x_i^2 & - \bar{x} \\ - \bar{x} & 1 \end{bmatrix}
    \end{align*}
    
\end{frame}

\begin{frame}{Question 4}

    Moreover,
    \begin{align*}
        R^2 &= \frac{\sum_{i=1}^n (\hat{y}_i - \bar{y})^2}{\sum_{i=1}^n (\hat{x}_i - \bar{x})^2}
        \\
        &= \hat{\beta} \frac{\sum_{i=1}^n (x_i - \bar{x})^2}{\sum_{i=1}^n (y_i - \bar{y})^2}
        \\
        &= 1 - \frac{SSR/(n-2)}{\sum_{i=1}^n (y_i - \bar{y})^2 / (n-1)}
        \\
        SSR &= (1 - R^2) \sum_{i=1}^n (y_i - \bar{y})^2
    \end{align*}
    
\end{frame}

